...뭔가 거하게 삽질만 하고 있는 거 같은데

src/study/Nemonuri.Study.CSharpSyntaxRewriter2.Modifier/Nemonuri.GreenNode.fst
@@ -9,6 +9,148 @@ type green_node_schema (#t:Type) = {
   children:(list (green_node_schema #t))
 }
 
+let is_valid_level_and_children_length (#t:Type) (gns:green_node_schema #t) : Tot bool =
+  if L.isEmpty gns.children then
+    gns.level = 0
+  else
+    gns.level > 0
+
+let has_type_green_leaf_schema (#t:Type) (gns:green_node_schema #t) : Tot bool =
+  (L.isEmpty gns.children) && 
+  (gns.level = 0) &&
+  (is_valid_level_and_children_length gns)
+let green_leaf_schema (#t:Type) = gns:green_node_schema #t{has_type_green_leaf_schema gns}
+
+
+let project_schema_level (#t:Type) (gns:green_node_schema #t) : Tot nat = gns.level
+
+let convert_green_node_schemas_to_levels (#t:Type) (l:list (green_node_schema #t))
+  : Tot (list nat)
+  = L.map (project_schema_level #t) l
+
+let get_max_level (#t:Type) (l:list (green_node_schema #t))
+  : Tot nat
+  = let nat_list = convert_green_node_schemas_to_levels l in
+    LT.max nat_list LT.default_int_comparer 0
+
+let has_type_green_branch_schema (#t:Type) (gns:green_node_schema #t) 
+  : Tot bool
+  = (not (L.isEmpty gns.children)) && 
+    (gns.level = (get_max_level gns.children) + 1) &&
+    (is_valid_level_and_children_length gns) &&
+    (L.for_all is_valid_level_and_children_length gns.children)
+let green_branch_schema (#t:Type) = gns:green_node_schema #t{has_type_green_branch_schema gns}
+
+(*
+let assert1 = assert (
+  forall (#t:Type) (gbs:green_branch_schema #t{gbs.level = 1}).
+    (L.for_all has_type_green_leaf_schema gbs.children)
+)
+*)
+
+(*
+let rec lemma1 (#t:Type) (gbs_hd:green_node_schema #t) (gbs_tl:(list (green_node_schema #t)))
+  : Lemma (ensures gbs_hd.level > 0 || has_type_green_leaf_schema gbs_hd )
+  = let children = gbs_hd.children in
+    match (children, gbs_tl) with
+    | ([], []) -> ()
+    | ([], hd::tl) -> lemma1 hd tl
+    | (hd::tl, []) -> lemma1 hd tl
+    | (hd1::tl1, hd2::tl2) -> lemma1 hd1 (L.append tl1 gbs_tl)
+*)
+
+type top_level_strict_green_node (#t:Type) : nat -> Type =
+  | Leaf : inner_leaf:green_leaf_schema #t -> top_level_strict_green_node #t inner_leaf.level
+  | Branch : inner_branch:green_branch_schema #t -> top_level_strict_green_node #t ( (get_max_level inner_branch.children) + 1 )
+
+type top_level_green_node (#t:Type) : nat -> Type =
+  | TLGN : strict_level:nat -> 
+         supplemented_level:nat ->
+         inner_top_level_strict_green_node:top_level_strict_green_node #t strict_level ->
+         top_level_green_node #t (strict_level + supplemented_level)
+
+let has_type_green_leaf_schema_or_green_branch_schema (#t:Type) (gns:green_node_schema #t)
+  : Tot bool
+  = (has_type_green_leaf_schema gns) || (has_type_green_branch_schema gns)
+
+let convert_to_top_level_strict_green_node 
+  (#t:Type)
+  (gns:green_node_schema #t{ 
+    (has_type_green_leaf_schema_or_green_branch_schema gns)
+  })
+  : Tot (top_level_strict_green_node #t gns.level) =
+  if has_type_green_branch_schema gns then
+    Branch gns
+  else
+    Leaf gns
+
+let loose_top_level_strict_green_node
+  (#t:Type) (#strict_level:nat) (tlsgn:top_level_strict_green_node #t strict_level)
+  (normal_level:nat{normal_level >= strict_level})
+  : top_level_green_node #t normal_level
+  = TLGN strict_level (normal_level - strict_level) tlsgn
+
+let rec has_type_green_node (#t:Type) (#limit_level:nat) (tlgn:top_level_green_node #t limit_level)
+  : Tot bool
+  = 
+
+(*
+let rec has_type_strict_green_node (#t:Type) (#n:nat) (tlsgn:top_level_strict_green_node #t n)
+  : Tot bool (decreases %[m;n])
+  = match tlsgn with
+  | Leaf _ -> true
+  | Branch inner_branch -> has_type_strict_green_node_for_list inner_branch.children
+and has_type_strict_green_node_for_list (#t:Type) (children:list (green_node_schema #t)) 
+  : Tot bool (decreases children)
+  = match children with
+  | [] -> true
+  | hd::tl ->
+    (has_type_green_leaf_schema_or_green_branch_schema hd) &&
+    (
+      let tlsgn = convert_to_top_level_strict_green_node hd in
+      has_type_strict_green_node tlsgn
+    ) &&
+    (has_type_strict_green_node_for_list tl)
+
+let convert_strict_green_node_to_normal 
+  (#t:Type) (#strict_level:nat) (sgn:strict_green_node #t strict_level)
+  (normal_level:nat{normal_level >= strict_level})
+  : green_node #t normal_level
+  = GN strict_level (normal_level - strict_level) sgn
+
+let project_level (#t:Type) (#n:nat) (gn:green_node #t n) : Tot nat =
+  let GN _ _ sgn = gn in
+  match sgn with
+  | Leaf inner_leaf -> inner_leaf.level
+  | Branch inner_branch -> inner_branch.level
+
+let project_value (#t:Type) (#n:nat) (gn:green_node #t n) : Tot t =
+  let GN _ _ sgn = gn in
+  match sgn with
+  | Leaf inner_leaf -> inner_leaf.value
+  | Branch inner_branch -> inner_branch.value
+*)
+
+(*
+let project_children (#t:Type) (#n:nat) (gn:green_node #t n) : Tot (list (green_node #t n)) =
+  let GN _ _ sgn = gn in
+  match sgn with
+  | Leaf _ -> []
+  | Branch inner_branch -> inner_branch.value
+*)
+
+(*
+let assert1 = assert (
+  forall (t:Type) (n:nat) (gn:green_node #t n).
+    match gn with
+    | Leaf v1 -> (v1.level = 0) /\ (v1.level = n)
+    | Branch v2 -> (v2.level = n)
+)
+*)
+
+
+
+(*
 let rec is_stratified (#t:Type) (gns:green_node_schema #t) : Tot bool =
   if gns.level = 0 then 
     L.isEmpty gns.children
@@ -28,6 +170,7 @@ let is_self_level_greater_then_children (#t:Type) (gns:green_node_schema #t) : T
     L.isEmpty gns.children
   else
     L.for_all (fun (gns2:green_node_schema #t) -> gns2.level < gns.level) gns.children
+*)
 
 (*
 let rec is_weakly_stratified (#t:Type) (gns:green_node_schema #t) 
@@ -40,6 +183,7 @@ let rec is_weakly_stratified (#t:Type) (gns:green_node_schema #t)
   )
 *)
 
+(*
 let rec is_weakly_stratified (#t:Type) (gns:green_node_schema #t) : Tot bool =
   if gns.level = 0 then 
     L.isEmpty gns.children
@@ -52,6 +196,7 @@ let rec is_weakly_stratified (#t:Type) (gns:green_node_schema #t) : Tot bool =
           L.for_all (fun (gns2:green_node_schema #t) -> is_weakly_stratified gns2) children
         else
           false
+*)
 
 (*
 let has_type_green_node (#t:Type) (gns:green_node_schema #t) : Tot bool = is_weakly_stratified gns
